MultiScalarMul_Abstract_Soundness.ec
@@ -8,16 +8,16 @@ require import BitEncoding StdBigop Bigalg.
 require import MultiScalarMul_Abstract MultiScalarMul_Abstract_Setup.
 require import IterationProps.
 
+
 section.
 
 declare module O <: OutCalls.
+declare axiom  O_lossless : islossless O.getU. 
 
-declare axiom O_lossless : islossless O.getU. 
-
-lemma multiscalarI_spec_ph argP args  argU : 
+lemma MSM_soundness_param_u_ph argP args  argU : 
  phoare [ MSM.multiScalarMulMain_Opt_Corrected : 
   arg = (argP, args, argU) 
-     ==>  res.`1 => res.`2 = (multiScalarMul_Simpl args argP T l)  ] = 1%r.
+     ==>  res.`1 => res.`2 = (multiScalarMul_Simpl args argP T l) ] = 1%r.
 proof.
 bypr.
 progress.
@@ -31,9 +31,8 @@ Pr[MSM.completeMain(P{m}, s{m}, U{m}) @ &m :
    res.`2 = multiScalarMul_Simpl args argP T l].
 byequiv (_: ={glob O} /\ arg{2} = (P{m}, s{m}, U{m}) /\ arg{1} = (P{m}, s{m}, U{m}) ==> res{2}.`1 => res{2}.`2 = res.`2{1} ).
 proc*.
-ecall (multieqs2 argP args argU).
-skip. progress. smt(). smt(). smt(). 
-auto.
+ecall (complete_optimized_equiv argP args argU).
+skip. progress. smt(). smt(). smt(). auto.
 smt().
 smt.
 auto. 
@@ -42,21 +41,22 @@ smt.
 qed.
 
 
-lemma multiscalar_spec_h argP args : 
- phoare [ MultiScalarMul(O).run : 
-  arg = (argP, args) 
-     ==>  res.`1 => res.`2 = (multiScalarMul_Simpl  args argP T l)  ] = 1%r .
+lemma MSM_soundness argP args &m : 
+ Pr[ MultiScalarMul(O).run(argP, args) @&m : 
+    res.`1 => res.`2 = (multiScalarMul_Simpl args argP T l) ] = 1%r.
+proof.
+byphoare (_:   arg = (argP, args)  ==> _).
 proc.
 seq 1 : #pre.
 call (_: true). auto.
 call (_: true). auto.
 apply O_lossless.
- auto.   
+auto.   
 exists* u_cand. elim*. move => u_candV.
-call (multiscalarI_spec_ph  argP args u_candV).
+call (MSM_soundness_param_u_ph argP args u_candV).
 wp.   skip. progress. 
-hoare. simplify. call(_:true). auto. auto.
- qed.   
+hoare. simplify. call(_:true). auto. auto. auto. auto.
+qed.   
 
 
 end section.
